Towards definition of translation

reform/translation.v
@@ -352,3 +352,30 @@ Proof.
     + now apply IHht6.
 Qed.
 
+(* We now will be defining what it is to be a translation for a context. *)
+Inductive ctx_trans : Env -> S.Env -> Prop :=
+| trans_nil  : ctx_trans nil nil
+| trans_cons : forall Γ Δ A B, ctx_trans Γ Δ -> ι B ~ A -> ctx_trans (A :: Γ) (B :: Δ)
+.
+
+(* And for term typing *)
+Inductive trans : (Env * Term * Term) -> (S.Env * S.Term * S.Term) -> Prop :=
+| trans_def : forall Γ a A Δ b B, ctx_trans Γ Δ -> ι b ~ a -> ι B ~ A -> trans (Γ,a,A) (Δ,b,B)
+.
+
+(* The next lemma is supposed to say that we can always chose a translation with a type
+   having the same head constructor. This has to be divided in several lemmata, one for each
+   type of constructor. *)
+
+Lemma trans_Π :
+  forall Γ a A1 A2 Δ b B, trans (Γ,a,Π A1 A2) (Δ,b,B) ->
+  exists B1 B2 c, trans (Γ,a,Π A1 A2) (Δ,c,S.Π B1 B2).
+Proof.
+  intros Γ a A1 A2 Δ b B h.
+Abort.
+
+
+
+
+
+
